src/tidy/rewrite_all.lean
@@ -1,0 +1,119 @@
+import data.list
+
+open tactic
+open interactive
+open interactive.types
+open expr
+open lean
+open lean.parser
+
+meta def rewrite_without_new_mvars (r : expr) (e : expr) (cfg : rewrite_cfg := {}) : tactic (expr × expr) :=
+do n_before ← num_goals,
+   (new_t, prf, metas) ← rewrite_core r e cfg,
+   try_apply_opt_auto_param cfg.to_apply_cfg metas,
+   n_after ← num_goals,
+   guard (n_before = n_after),
+   return (new_t, prf)
+
+meta def each_goal {α} (t : conv α) : conv (list α) := sorry
+
+
+open tactic.interactive
+
+meta def search_attribute : user_attribute := {
+  name := `search,
+  descr := ""
+}
+
+run_cmd attribute.register `search_attribute
+
+meta inductive expr_lens
+| app_fun : expr_lens → expr → expr_lens
+| app_arg : expr_lens → expr → expr_lens
+| entire  : expr_lens
+
+open expr_lens
+
+meta def expr_lens.replace : expr_lens → expr → expr
+| (app_fun l f) x := expr_lens.replace l (expr.app f x)
+| (app_arg l x) f := expr_lens.replace l (expr.app f x)
+| entire        e := e 
+
+meta def expr_lens.congr : expr_lens → expr → tactic expr
+| (app_fun l f) x_eq := do fx_eq ← mk_congr_arg f x_eq,
+                                     expr_lens.congr l fx_eq
+| (app_arg l x) f_eq := do fx_eq ← mk_congr_fun f_eq x,
+                                     expr_lens.congr l fx_eq
+| entire                  e_eq := pure e_eq
+
+-- meta inductive expr_lens
+-- | app : expr_lens → expr → ℕ → list expr → expr_lens -- with arguments l f i a, this focuses `l` on the `i`-th argument of `f`, with other arguments provided by `a`.
+-- | entire : expr_lens
+
+-- open expr_lens
+
+-- meta def expr_lens.replace : expr_lens → expr → expr
+-- | (app l f i a) e := sorry
+-- | entire        e := e
+
+meta def rewrite_fold_aux {α} (F : expr_lens → expr → α → tactic α) : expr_lens → expr → α → tactic α 
+| l e a := (do a' ← F l e a,
+              match e with
+              | (expr.app f x) := do a_f ← rewrite_fold_aux (expr_lens.app_arg l x) f a',
+                                            rewrite_fold_aux (expr_lens.app_fun l f) x a_f
+              | _ := pure a'
+              end) <|> pure a
+. 
+
+meta def rewrite_fold {α} (F : expr_lens → expr → α → tactic α) (e : expr) (a : α) : tactic α := rewrite_fold_aux F expr_lens.entire e a
+
+meta def rewrite_F (r : expr × bool) (l : expr_lens) (e : expr) (state : list (expr × expr)) : tactic (list (expr × expr)) := 
+do 
+  (v, pr) ← rewrite_without_new_mvars r.1 e {symm := r.2},
+  let v' := l.replace v,
+  pr' ← l.congr pr,
+  pure ((v', pr') :: state)
+
+def remove_adjacent_duplicates {α β} (f : α → β) [decidable_eq β] : list α → list α
+| (x :: y :: t) := if f x = f y then
+                     remove_adjacent_duplicates (y :: t)
+                   else
+                     x :: (remove_adjacent_duplicates (y :: t))
+| [x] := [x]
+| [] := []
+
+meta def all_rewrites (r : expr × bool) (e : expr) : tactic (list (expr × expr)) :=
+do results ← rewrite_fold (rewrite_F r) e [],
+   let results : list (expr × expr) := remove_adjacent_duplicates (λ p, p.1) results,
+  --  tactic.trace results,
+   pure results
+
+meta def perform_nth_rewrite (r : expr × bool) (n : ℕ) : tactic unit := 
+do e ← target,
+   rewrites ← all_rewrites r e,
+   (new_t, prf) ← rewrites.nth n,
+   replace_target new_t prf
+
+-- TODO interactive version
+
+meta def all_rewrites_using (a : name) (e : expr) : tactic (list (expr × expr)) :=
+do names ← attribute.get_instances a,
+   rules ← names.mmap $ mk_const,
+   let pairs := rules.map (λ e, (e, ff)) ++ rules.map (λ e, (e, tt)),
+   results ← pairs.mmap $ λ r, all_rewrites r e,
+   pure results.join
+
+meta def perform_nth_rewrite_using (a : name) (n : ℕ) : tactic unit := 
+do e ← target,
+   rewrites ← all_rewrites_using a e,
+   (new_t, prf) ← rewrites.nth n,
+   replace_target new_t prf
+
+@[search] lemma b (l : list ℕ) : 1 :: l = 2 :: l := sorry
+
+example (f : ℕ → list ℕ → Type) : f 3 [1,1,1,2,1] = f 3 [1,2,1,2,1] :=
+begin
+target >>= all_rewrites_using `search,
+perform_nth_rewrite_using `search 5,
+refl
+end
